refactor definitions and lemmas into library

lib/binaryTree.dfy
@@ -1,237 +1,895 @@
 include "../lib/seq.dfy"
 
 module BinaryTree {
-import opened Seq
-datatype Tree = Node(val: int, left: Tree, right: Tree) | Nil
+    import opened Seq
 
-function TreePreorderTraversal(root: Tree): seq<Tree>
-    // ensures forall x :: x in TreePreorderTraversal(root) ==> x != Nil
-    // ensures forall x :: x in TreePreorderTraversal(root) ==> x != Nil && (x == root || x in TreePreorderTraversal(root.left) || x in TreePreorderTraversal(root.right))
-    // ensures forall x :: x in root.repr ==> x in PreorderTraversal(root)
-    // ensures injectiveSeq(TreePreorderTraversal(root))
-    // ensures forall k :: 0 <= k < |TreePreorderTraversal(root)| ==> TreePreorderTraversal(root)[k] in root.repr
-    // ensures forall k :: 0 <= k < |PreorderTraversal(root)| ==> forall child :: child in PreorderTraversal(root)[k].repr && child != child in PreorderTraversal(root)[k] ==> exists j :: k < j < |PreorderTraversal(root)| && PreorderTraversal(root)[j] == child
-{
-   if root == Nil then [] else if root.left != Nil && root.right != Nil then [root]+TreePreorderTraversal(root.left)+TreePreorderTraversal(root.right) else if root.left != Nil then [root]+TreePreorderTraversal(root.left) else if root.right != Nil then [root]+TreePreorderTraversal(root.right) else [root]
-}
+    //Definitions
+    datatype Tree = Node(val: int, left: Tree, right: Tree) | Nil
 
-predicate validTree(root: Tree) {
-    if root != Nil then root.left != root && root.right != root && (forall lchild :: lchild in TreePreorderTraversal(root.left) ==> lchild != root && lchild !in TreePreorderTraversal(root.right)) && (forall rchild :: rchild in TreePreorderTraversal(root.right) ==> rchild != root && rchild !in TreePreorderTraversal(root.left)) && validTree(root.right) && validTree(root.left) else true
-    // if root != Nil then root.left != root && root.right != root && root !in TreePreorderTraversal(root.left)  && root !in TreePreorderTraversal(root.right) && forall x :: x in TreePreorderTraversal(root.left) ==> x !in TreePreorderTraversal(root.right) && forall x :: x in TreePreorderTraversal(root.right) ==> x !in TreePreorderTraversal(root.left) && validTree(root.right) && validTree(root.left) else true
-}
+    function TreePreorderTraversal(root: Tree): seq<Tree>
+        // ensures forall x :: x in TreePreorderTraversal(root) ==> x != Nil
+        // ensures forall x :: x in TreePreorderTraversal(root) ==> x != Nil && (x == root || x in TreePreorderTraversal(root.left) || x in TreePreorderTraversal(root.right))
+        // ensures forall x :: x in root.repr ==> x in PreorderTraversal(root)
+        // ensures injectiveSeq(TreePreorderTraversal(root))
+        // ensures forall k :: 0 <= k < |TreePreorderTraversal(root)| ==> TreePreorderTraversal(root)[k] in root.repr
+        // ensures forall k :: 0 <= k < |PreorderTraversal(root)| ==> forall child :: child in PreorderTraversal(root)[k].repr && child != child in PreorderTraversal(root)[k] ==> exists j :: k < j < |PreorderTraversal(root)| && PreorderTraversal(root)[j] == child
+    {
+    if root == Nil then [] else if root.left != Nil && root.right != Nil then [root]+TreePreorderTraversal(root.left)+TreePreorderTraversal(root.right) else if root.left != Nil then [root]+TreePreorderTraversal(root.left) else if root.right != Nil then [root]+TreePreorderTraversal(root.right) else [root]
+    }
 
-lemma rootNotInChildren(root: Tree)
-    requires root != Nil
-    requires validTree(root);
-    ensures root != Nil && root.left != Nil ==> root !in TreePreorderTraversal(root.left)
-    ensures root != Nil && root.right != Nil ==> root !in TreePreorderTraversal(root.right)
-{
-    assert root in TreePreorderTraversal(root);
-    tpt(root);
-    if root != Nil && root.left != Nil && root.right != Nil {
+    predicate validTree(root: Tree) {
+        if root != Nil then root.left != root && root.right != root && (forall lchild :: lchild in TreePreorderTraversal(root.left) ==> lchild != root && lchild !in TreePreorderTraversal(root.right)) && (forall rchild :: rchild in TreePreorderTraversal(root.right) ==> rchild != root && rchild !in TreePreorderTraversal(root.left)) && validTree(root.right) && validTree(root.left) else true
+        // if root != Nil then root.left != root && root.right != root && root !in TreePreorderTraversal(root.left)  && root !in TreePreorderTraversal(root.right) && forall x :: x in TreePreorderTraversal(root.left) ==> x !in TreePreorderTraversal(root.right) && forall x :: x in TreePreorderTraversal(root.right) ==> x !in TreePreorderTraversal(root.left) && validTree(root.right) && validTree(root.left) else true
+    }
+
+    function max(left: int, right: int): int {
+        if left > right then left else right
+    }
+
+    function TreeSet(root: Tree): set<Tree> {
+        match root {
+            case Nil => {}
+            case Node(val, left, right) => {root}+TreeSet(left)+TreeSet(right)
+        }
+    }
+
+    function TreeHeight(root: Tree): int 
+        ensures TreeHeight(root) >= -1
+    {
+        if root == Nil then -1 else if root.left == Nil && root.right == Nil then 0 else max(TreeHeight(root.left), TreeHeight(root.right)) + 1
+    }
+
+    predicate isChild(a: Tree, b: Tree) {
+        a != Nil && (a.left == b || a.right == b)
+    }
+
+    predicate isParentOrChild(a: Tree, b: Tree) {
+        //a != Nil && b != Nil && (a.left == b || a.right == b || (a == b.left || a == b.right))
+        a != Nil && b != Nil && (isChild(a, b) || isChild(b, a))
+    }
+
+    predicate isTreePath(path: seq<Tree>, start: Tree, end: Tree) {
+        if |path| == 0 then false else if |path| == 1 then start != Nil && start == end && path[0] == start else match path[0] {
+            case Nil => false
+            case Node(val, left, right) => path[0] == start && path[|path|-1] == end && isParentOrChild(path[0], path[1]) && isTreePath(path[1..], path[1], end)
+        }
+    }
+
+    predicate isTreePathAlt(path: seq<Tree>, start: Tree, end: Tree) {
+        if |path| == 0 then false else if |path| == 1 then start != Nil && start == end && path[0] == start else path[0] == start && start != Nil && end == path[|path|-1] == end && forall i :: 0 <= i < |path| - 1 ==> isParentOrChild(path[i], path[i+1])
+    }
+
+    predicate isDescTreePath(path: seq<Tree>, start: Tree, end: Tree) {
+        if |path| == 0 then false else if |path| == 1 then match path[0] {
+                case Nil => false
+                case Node(val, left, right) => path[0] == start && end == start
+        } else match path[0] {
+            case Nil => false
+            case Node(val, left, right) => end != Nil && path[|path|-1] == end && path[0] == start && path[1] != Nil && ((left == path[1] && isDescTreePath(path[1..],left, end)) || (right == path[1] && isDescTreePath(path[1..], right, end)))
+        }
+    }
+
+    predicate isAscTreePath(paths: seq<Tree>, start: Tree, end: Tree) {
+        if |paths| == 0 then false else if |paths| == 1 then match paths[0] {
+            case Nil => false
+            case Node(val, left, right) => start == paths[0] && end == start
+        } else match paths[0] {
+            case Nil => false
+            case Node(val, left, right) => end != Nil && paths[|paths|-1] == end && start == paths[0] && paths[1] != Nil  && ((paths[0] == paths[1].left && isAscTreePath(paths[1..], paths[1], end)) || (paths[0] == paths[1].right && isAscTreePath(paths[1..], paths[1], end)))
+        }
+    }
+
+    ghost predicate ChildrenAreSeparate(root: Tree) {
+        root == Nil || (root != Nil && (TreeSet(root.left) !! TreeSet(root.right)) && ChildrenAreSeparate(root.left) && ChildrenAreSeparate(root.right))
+    }
+
+    predicate isValidPath(path: seq<Tree>, root: Tree) {
+        forall node :: node in path ==> node in TreeSet(root)
+    }
+
+    ghost predicate isPath(path: seq<Tree>, start: Tree, end: Tree, root: Tree) {
+        isTreePath(path,start, end) && isValidPath(path, root) && distinct(path)
+    }
+
+    predicate isLeaf(node: Tree ) {
+        node != Nil && node.right == Nil && node.left == Nil
+    }
+
+    //lemmas
+
+    lemma rootNotInChildren(root: Tree)
+        requires root != Nil
+        requires validTree(root);
+        ensures root != Nil && root.left != Nil ==> root !in TreePreorderTraversal(root.left)
+        ensures root != Nil && root.right != Nil ==> root !in TreePreorderTraversal(root.right)
+    {
+        assert root in TreePreorderTraversal(root);
+        tpt(root);
+        if root != Nil && root.left != Nil && root.right != Nil {
+            calc {
+                TreePreorderTraversal(root);
+                [root]+TreePreorderTraversal(root.left)+TreePreorderTraversal(root.right);
+            }
+            assert root !in TreePreorderTraversal(root.left);
+        }else{
+
+        }
+    }
+
+    lemma {:verify } TPTInjective(root: Tree) 
+        requires validTree(root)
+        requires root != Nil
+        ensures distinct(TreePreorderTraversal(root))
+    {
+        NoNil(root);
+        tpt(root);
+        assert root !in TreePreorderTraversal(root.left);
+        assert root !in TreePreorderTraversal(root.right);
+        if root.right != Nil && root.left != Nil {
+            calc{
+                TreePreorderTraversal(root);
+                [root]+TreePreorderTraversal(root.left)+TreePreorderTraversal(root.right);
+            }
+            TPTInjective(root.left);
+            TPTInjective(root.right);
+            distincts([root], TreePreorderTraversal(root.left));
+            distincts([root] + TreePreorderTraversal(root.left), TreePreorderTraversal(root.right));
+
+        }else if root.right != Nil {
+            calc{
+                TreePreorderTraversal(root);
+                [root]+TreePreorderTraversal(root.right);
+            }
+            TPTInjective(root.right);
+            distincts([root], TreePreorderTraversal(root.right));
+        }else if root.left != Nil {
+
+            calc{
+                TreePreorderTraversal(root);
+                [root]+TreePreorderTraversal(root.left);
+            }
+            TPTInjective(root.left);
+            distincts([root], TreePreorderTraversal(root.left));
+        }
+    }
+
+    lemma NoNil(root: Tree)
+        ensures forall x :: x in TreePreorderTraversal(root) ==> x != Nil
+    {
+
+    }
+
+    lemma tpt(root: Tree)
+        ensures forall x :: x in TreePreorderTraversal(root) ==> x != Nil
+        ensures forall x :: x in TreePreorderTraversal(root) ==> x != Nil && (x == root || x in TreePreorderTraversal(root.left) || x in TreePreorderTraversal(root.right))
+    {
+
+    }
+
+
+    lemma AllChildTraversalElementsInRoot(root: Tree, elem: Tree)
+        requires elem in TreePreorderTraversal(root)
+        ensures forall child :: child in TreePreorderTraversal(elem) ==> child in TreePreorderTraversal(root)
+    {
+
+    }
+
+    lemma TreePreorderTraversalSubstrings(root: Tree)
+        requires root != Nil
+        ensures root.left != Nil ==> isSubstring(TreePreorderTraversal(root.left), TreePreorderTraversal(root))
+        ensures root.right != Nil ==> isSubstring(TreePreorderTraversal(root.right), TreePreorderTraversal(root))
+    {
+    if root.left != Nil && root.right != Nil {
         calc {
             TreePreorderTraversal(root);
             [root]+TreePreorderTraversal(root.left)+TreePreorderTraversal(root.right);
         }
-        assert root !in TreePreorderTraversal(root.left);
-    }else{
+        var k := 1;
+        var j := |TreePreorderTraversal(root.left)|+1;
+        assert 0 <= k <= j <= |TreePreorderTraversal(root)| && TreePreorderTraversal(root.left) == TreePreorderTraversal(root)[1..|TreePreorderTraversal(root.left)|+1];
 
-    }
-}
-
-lemma {:verify } TPTInjective(root: Tree) 
-    requires validTree(root)
-    requires root != Nil
-    ensures distinct(TreePreorderTraversal(root))
-{
-    NoNil(root);
-    tpt(root);
-    assert root !in TreePreorderTraversal(root.left);
-    assert root !in TreePreorderTraversal(root.right);
-    if root.right != Nil && root.left != Nil {
-        calc{
-            TreePreorderTraversal(root);
-            [root]+TreePreorderTraversal(root.left)+TreePreorderTraversal(root.right);
-        }
-        TPTInjective(root.left);
-        TPTInjective(root.right);
-        distincts([root], TreePreorderTraversal(root.left));
-        distincts([root] + TreePreorderTraversal(root.left), TreePreorderTraversal(root.right));
-
-    }else if root.right != Nil {
-        calc{
-            TreePreorderTraversal(root);
-            [root]+TreePreorderTraversal(root.right);
-        }
-        TPTInjective(root.right);
-        distincts([root], TreePreorderTraversal(root.right));
-    }else if root.left != Nil {
-
-        calc{
+        var s := 1+|TreePreorderTraversal(root.left)|;
+        var t := |TreePreorderTraversal(root)|;
+        assert 0 <= s <= t <= |TreePreorderTraversal(root)| && TreePreorderTraversal(root.right) == TreePreorderTraversal(root)[s..t];
+    }else if root.left != Nil && root.right == Nil {
+        calc {
             TreePreorderTraversal(root);
             [root]+TreePreorderTraversal(root.left);
         }
-        TPTInjective(root.left);
-        distincts([root], TreePreorderTraversal(root.left));
+        var k := 1;
+        var j := |TreePreorderTraversal(root.left)|+1;
+        assert 0 <= k <= j <= |TreePreorderTraversal(root)| && TreePreorderTraversal(root.left) == TreePreorderTraversal(root)[1..j];
+    }else if root.left == Nil && root.right != Nil {
+        calc {
+            TreePreorderTraversal(root);
+            [root]+TreePreorderTraversal(root.right);
+        }
+        var k := 1;
+        var j := |TreePreorderTraversal(root.right)|+1;
+        assert 0 <= k <= j <= |TreePreorderTraversal(root)| && TreePreorderTraversal(root.right) == TreePreorderTraversal(root)[1..j];
     }
-}
-
-lemma NoNil(root: Tree)
-    ensures forall x :: x in TreePreorderTraversal(root) ==> x != Nil
-{
-
-}
-
-lemma tpt(root: Tree)
-    ensures forall x :: x in TreePreorderTraversal(root) ==> x != Nil
-    ensures forall x :: x in TreePreorderTraversal(root) ==> x != Nil && (x == root || x in TreePreorderTraversal(root.left) || x in TreePreorderTraversal(root.right))
-{
-
-}
-
-
-lemma AllChildTraversalElementsInRoot(root: Tree, elem: Tree)
-    requires elem in TreePreorderTraversal(root)
-    ensures forall child :: child in TreePreorderTraversal(elem) ==> child in TreePreorderTraversal(root)
-{
-
-}
-
-lemma TreePreorderTraversalSubstrings(root: Tree)
-    requires root != Nil
-    ensures root.left != Nil ==> isSubstring(TreePreorderTraversal(root.left), TreePreorderTraversal(root))
-    ensures root.right != Nil ==> isSubstring(TreePreorderTraversal(root.right), TreePreorderTraversal(root))
-{
-   if root.left != Nil && root.right != Nil {
-    calc {
-        TreePreorderTraversal(root);
-        [root]+TreePreorderTraversal(root.left)+TreePreorderTraversal(root.right);
     }
-    var k := 1;
-    var j := |TreePreorderTraversal(root.left)|+1;
-    assert 0 <= k <= j <= |TreePreorderTraversal(root)| && TreePreorderTraversal(root.left) == TreePreorderTraversal(root)[1..|TreePreorderTraversal(root.left)|+1];
 
-    var s := 1+|TreePreorderTraversal(root.left)|;
-    var t := |TreePreorderTraversal(root)|;
-    assert 0 <= s <= t <= |TreePreorderTraversal(root)| && TreePreorderTraversal(root.right) == TreePreorderTraversal(root)[s..t];
-   }else if root.left != Nil && root.right == Nil {
-    calc {
-        TreePreorderTraversal(root);
-        [root]+TreePreorderTraversal(root.left);
-    }
-    var k := 1;
-    var j := |TreePreorderTraversal(root.left)|+1;
-    assert 0 <= k <= j <= |TreePreorderTraversal(root)| && TreePreorderTraversal(root.left) == TreePreorderTraversal(root)[1..j];
-   }else if root.left == Nil && root.right != Nil {
-    calc {
-        TreePreorderTraversal(root);
-        [root]+TreePreorderTraversal(root.right);
-    }
-    var k := 1;
-    var j := |TreePreorderTraversal(root.right)|+1;
-    assert 0 <= k <= j <= |TreePreorderTraversal(root)| && TreePreorderTraversal(root.right) == TreePreorderTraversal(root)[1..j];
-   }
-}
-
-lemma AllContained(root: Tree)
-    requires root != Nil
-    ensures forall x :: x in TreePreorderTraversal(root) ==> (x == root || x in TreePreorderTraversal(root.left) || x in TreePreorderTraversal(root.right))
-{
-}
-
-lemma {:verify true} {:induction false} AllChildrenTraversalsAreSubstrings(root: Tree) 
-    requires root != Nil
-    ensures forall x ::x in TreePreorderTraversal(root) ==> isSubstring(TreePreorderTraversal(x), TreePreorderTraversal(root))
-{
-    NoNil(root);
-    AllContained(root);
-    forall x | x in TreePreorderTraversal(root) 
-        ensures isSubstring(TreePreorderTraversal(x), TreePreorderTraversal(root))
+    lemma AllContained(root: Tree)
+        requires root != Nil
+        ensures forall x :: x in TreePreorderTraversal(root) ==> (x == root || x in TreePreorderTraversal(root.left) || x in TreePreorderTraversal(root.right))
     {
-        tpt(root);
-        if x == root {
-            var k, j := 0, |TreePreorderTraversal(root)|;
-            assert 0 <= k <= j <= |TreePreorderTraversal(root)| && TreePreorderTraversal(root) == TreePreorderTraversal(root)[k..j];
-        }else if x == root.left || x == root.right {
-           TreePreorderTraversalSubstrings(root); 
-        }else {
-            if root.left != Nil && root.right != Nil {
-                assert x != root;
-                assert TreePreorderTraversal(root) == [root] + TreePreorderTraversal(root.left) + TreePreorderTraversal(root.right);
-                if root.left != Nil  && x in TreePreorderTraversal(root.left) {
+    }
+
+    lemma {:induction false} AllChildrenTraversalsAreSubstrings(root: Tree) 
+        requires root != Nil
+        ensures forall x ::x in TreePreorderTraversal(root) ==> isSubstring(TreePreorderTraversal(x), TreePreorderTraversal(root))
+    {
+        NoNil(root);
+        AllContained(root);
+        forall x | x in TreePreorderTraversal(root) 
+            ensures isSubstring(TreePreorderTraversal(x), TreePreorderTraversal(root))
+        {
+            tpt(root);
+            if x == root {
+                var k, j := 0, |TreePreorderTraversal(root)|;
+                assert 0 <= k <= j <= |TreePreorderTraversal(root)| && TreePreorderTraversal(root) == TreePreorderTraversal(root)[k..j];
+            }else if x == root.left || x == root.right {
+            TreePreorderTraversalSubstrings(root); 
+            }else {
+                if root.left != Nil && root.right != Nil {
+                    assert x != root;
+                    assert TreePreorderTraversal(root) == [root] + TreePreorderTraversal(root.left) + TreePreorderTraversal(root.right);
+                    if root.left != Nil  && x in TreePreorderTraversal(root.left) {
+                        AllChildrenTraversalsAreSubstrings(root.left);
+                        assert isSubstring(TreePreorderTraversal(x), TreePreorderTraversal(root.left));
+                        TreePreorderTraversalSubstrings(root);
+                        AllSubstringsAreSubstrings(TreePreorderTraversal(x), TreePreorderTraversal(root.left), TreePreorderTraversal(root));
+                    }
+                    if root.right != Nil && x in TreePreorderTraversal(root.right) {
+                        AllChildrenTraversalsAreSubstrings(root.right);
+                        assert isSubstring(TreePreorderTraversal(x), TreePreorderTraversal(root.right));
+                        TreePreorderTraversalSubstrings(root);
+                        AllSubstringsAreSubstrings(TreePreorderTraversal(x), TreePreorderTraversal(root.right), TreePreorderTraversal(root));
+                    }
+                }else if root.left != Nil  && x in TreePreorderTraversal(root.left) {
                     AllChildrenTraversalsAreSubstrings(root.left);
                     assert isSubstring(TreePreorderTraversal(x), TreePreorderTraversal(root.left));
-                    TreePreorderTraversalSubstrings(root);
-                    AllSubstringsAreSubstrings(TreePreorderTraversal(x), TreePreorderTraversal(root.left), TreePreorderTraversal(root));
-                }
-                if root.right != Nil && x in TreePreorderTraversal(root.right) {
+                        TreePreorderTraversalSubstrings(root);
+                        AllSubstringsAreSubstrings(TreePreorderTraversal(x), TreePreorderTraversal(root.left), TreePreorderTraversal(root));
+                }else  if root.right != Nil && x in TreePreorderTraversal(root.right) {
                     AllChildrenTraversalsAreSubstrings(root.right);
-                    assert isSubstring(TreePreorderTraversal(x), TreePreorderTraversal(root.right));
-                    TreePreorderTraversalSubstrings(root);
-                    AllSubstringsAreSubstrings(TreePreorderTraversal(x), TreePreorderTraversal(root.right), TreePreorderTraversal(root));
+                        assert isSubstring(TreePreorderTraversal(x), TreePreorderTraversal(root.right));
+                        TreePreorderTraversalSubstrings(root);
+                        AllSubstringsAreSubstrings(TreePreorderTraversal(x), TreePreorderTraversal(root.right), TreePreorderTraversal(root));
+                }else{
+                    assert x != root;
+                    assert x !in TreePreorderTraversal(root.left);
+                    assert x !in TreePreorderTraversal(root.right);
+                    assert false;
                 }
-            }else if root.left != Nil  && x in TreePreorderTraversal(root.left) {
-                AllChildrenTraversalsAreSubstrings(root.left);
-                assert isSubstring(TreePreorderTraversal(x), TreePreorderTraversal(root.left));
-                    TreePreorderTraversalSubstrings(root);
-                    AllSubstringsAreSubstrings(TreePreorderTraversal(x), TreePreorderTraversal(root.left), TreePreorderTraversal(root));
-            }else  if root.right != Nil && x in TreePreorderTraversal(root.right) {
-                AllChildrenTraversalsAreSubstrings(root.right);
-                    assert isSubstring(TreePreorderTraversal(x), TreePreorderTraversal(root.right));
-                    TreePreorderTraversalSubstrings(root);
-                    AllSubstringsAreSubstrings(TreePreorderTraversal(x), TreePreorderTraversal(root.right), TreePreorderTraversal(root));
-            }else{
-                assert x != root;
-                assert x !in TreePreorderTraversal(root.left);
-                assert x !in TreePreorderTraversal(root.right);
-                assert false;
             }
         }
     }
-}
 
-lemma TreeChildrenAreLater(root: Tree)
-    requires root != Nil
-    ensures forall x :: x in TreePreorderTraversal(root) && x != root ==> exists k:nat :: 0 < k < |TreePreorderTraversal(root)| && TreePreorderTraversal(root)[k] == x
-{
-    NoNil(root);
-}
-
-lemma {:verify true} TreePreorderTraversalChildrenAreLater3(root: Tree, elem: Tree, k: nat) 
-    // requires validTree(root)
-    requires distinct(TreePreorderTraversal(root))
-    requires k < |TreePreorderTraversal(root)|
-    requires elem in TreePreorderTraversal(root)
-    requires elem != Nil
-    requires TreePreorderTraversal(root)[k] == elem
-    ensures forall child :: child in TreePreorderTraversal(elem) && child != elem ==> exists j: nat :: k < j < |TreePreorderTraversal(root)| && TreePreorderTraversal(root)[j] == child
-{
-    // TPTInjective(root);
-    AllChildTraversalElementsInRoot(root, elem);
-    AllChildrenTraversalsAreSubstrings(root);
-    AllChildrenTraversalsAreSubstrings(elem);
-    TreeChildrenAreLater(elem);
-    forall child | child in TreePreorderTraversal(elem) && child != elem
-        ensures exists j: nat :: k < j < |TreePreorderTraversal(root)| && TreePreorderTraversal(root)[j] == child
+    lemma TreeChildrenAreLater(root: Tree)
+        requires root != Nil
+        ensures forall x :: x in TreePreorderTraversal(root) && x != root ==> exists k:nat :: 0 < k < |TreePreorderTraversal(root)| && TreePreorderTraversal(root)[k] == x
     {
-        assert child in TreePreorderTraversal(root);
-        assert child != elem;
-        var j:nat :| 0 < j < |TreePreorderTraversal(elem)| && TreePreorderTraversal(elem)[j] == child;
-        var s,t :| 0 <= s < t <= |TreePreorderTraversal(root)| && TreePreorderTraversal(elem) == TreePreorderTraversal(root)[s..t];
-        assert TreePreorderTraversal(root)[k] == elem;
-        assert TreePreorderTraversal(elem)[0] == elem;
-        assert TreePreorderTraversal(root)[s] == elem;
-        assert s == k;
-        assert TreePreorderTraversal(root)[s+j] == child;
-
-        // seqbusiness(TreePreorderTraversal(root), child);
-        // var j :| 0 <= j < |TreePreorderTraversal(root)| && TreePreorderTraversal(root)[j] == child;
-        // assert isSubstring(TreePreorderTraversal(child), TreePreorderTraversal(elem));
-        // AllSubstringsAreSubstrings(TreePreorderTraversal(child), TreePreorderTraversal(elem), TreePreorderTraversal(root));
-        // assert isSubstring(TreePreorderTraversal(child), TreePreorderTraversal(root));
-        // // assert |TreePreorderTraversal(child)| <= |TreePreorderTraversal(elem)|;
-        // var s,t :| 0 <= s < t <= |TreePreorderTraversal(root)| && TreePreorderTraversal(child) == TreePreorderTraversal(root)[s..t];
-        // assert j == s;
+        NoNil(root);
     }
-}
+
+    lemma TreePreorderTraversalChildrenAreLater3(root: Tree, elem: Tree, k: nat) 
+        requires distinct(TreePreorderTraversal(root))
+        requires k < |TreePreorderTraversal(root)|
+        requires elem in TreePreorderTraversal(root)
+        requires elem != Nil
+        requires TreePreorderTraversal(root)[k] == elem
+        ensures forall child :: child in TreePreorderTraversal(elem) && child != elem ==> exists j: nat :: k < j < |TreePreorderTraversal(root)| && TreePreorderTraversal(root)[j] == child
+    {
+        // TPTInjective(root);
+        AllChildTraversalElementsInRoot(root, elem);
+        AllChildrenTraversalsAreSubstrings(root);
+        AllChildrenTraversalsAreSubstrings(elem);
+        TreeChildrenAreLater(elem);
+        forall child | child in TreePreorderTraversal(elem) && child != elem
+            ensures exists j: nat :: k < j < |TreePreorderTraversal(root)| && TreePreorderTraversal(root)[j] == child
+        {
+            assert child in TreePreorderTraversal(root);
+            assert child != elem;
+            var j:nat :| 0 < j < |TreePreorderTraversal(elem)| && TreePreorderTraversal(elem)[j] == child;
+            var s,t :| 0 <= s < t <= |TreePreorderTraversal(root)| && TreePreorderTraversal(elem) == TreePreorderTraversal(root)[s..t];
+            assert TreePreorderTraversal(root)[k] == elem;
+            assert TreePreorderTraversal(elem)[0] == elem;
+            assert TreePreorderTraversal(root)[s] == elem;
+            assert s == k;
+            assert TreePreorderTraversal(root)[s+j] == child;
+
+            // seqbusiness(TreePreorderTraversal(root), child);
+            // var j :| 0 <= j < |TreePreorderTraversal(root)| && TreePreorderTraversal(root)[j] == child;
+            // assert isSubstring(TreePreorderTraversal(child), TreePreorderTraversal(elem));
+            // AllSubstringsAreSubstrings(TreePreorderTraversal(child), TreePreorderTraversal(elem), TreePreorderTraversal(root));
+            // assert isSubstring(TreePreorderTraversal(child), TreePreorderTraversal(root));
+            // // assert |TreePreorderTraversal(child)| <= |TreePreorderTraversal(elem)|;
+            // var s,t :| 0 <= s < t <= |TreePreorderTraversal(root)| && TreePreorderTraversal(child) == TreePreorderTraversal(root)[s..t];
+            // assert j == s;
+        }
+    }
+
+
+    lemma TreeHeightMax(root: Tree) 
+        ensures forall node :: node in TreeSet(root) ==> TreeHeight(root) >= TreeHeight(node)
+    {}
+
+    lemma TreePathsAreTheSameAlt(path: seq<Tree>, start: Tree, end: Tree)
+        requires start != Nil
+        requires end != Nil
+        requires isTreePath(path, start, end)
+        ensures isTreePathAlt(path, start, end)
+    {
+
+    }
+
+    lemma TreePathsAreTheSame(path: seq<Tree>, start: Tree, end: Tree)
+        requires start != Nil
+        requires end != Nil
+        requires isTreePathAlt(path, start, end)
+        ensures isTreePath(path, start, end)
+    {
+
+    }
+
+    lemma DescPathChildren(path: seq<Tree>, start: Tree, end: Tree)
+        requires start != Nil
+        requires end != Nil
+        requires |path| > 1
+        requires isDescTreePath(path, start, end)
+        ensures forall i :: 0 <= i < |path| - 1 ==> isChild(path[i], path[i+1])
+    {
+    }
+
+    lemma DescPathChildrenAlt(path: seq<Tree>, start: Tree, end: Tree)
+        requires start != Nil
+        requires end != Nil
+        requires |path| > 1
+        requires path[0] == start;
+        requires path[|path|-1] == end;
+        requires forall i :: 0 <= i < |path| ==> path[i] != Nil
+        requires forall i :: 0 <= i < |path| - 1 ==> isChild(path[i], path[i+1])
+        ensures isDescTreePath(path, start, end)
+    {
+    }
+
+    lemma TreePathChildrenAlt(path: seq<Tree>, start: Tree, end: Tree) 
+        requires start != Nil
+        requires end != Nil
+        requires |path| >= 1
+        requires path[0] == start;
+        requires path[|path|-1] == end;
+        requires forall i :: 0 <= i < |path| ==> path[i] != Nil
+        requires forall i :: 0 <= i < |path| - 1 ==> isParentOrChild(path[i], path[i+1])
+        ensures isTreePath(path, start, end)
+    {
+
+    }
+
+    lemma DescPathChildrenReverse(path: seq<Tree>, start: Tree, end: Tree)
+        requires start != Nil
+        requires end != Nil
+        requires |path| > 1
+        requires isDescTreePath(path, start, end)
+        ensures forall i :: 0 <= i < |reverse(path)| - 1 ==> isChild(reverse(path)[i+1], reverse(path)[i])
+    {
+        DescPathChildren(path, start, end);
+        ReverseIndexAll(path);
+    }
+
+    lemma AscPathChildrenAlt(path: seq<Tree>, start: Tree, end: Tree)
+        requires start != Nil
+        requires end != Nil
+        requires |path| > 1
+        requires path[0] == start;
+        requires path[|path|-1] == end;
+        requires forall i :: 0 <= i < |path| - 1 ==> isChild(path[i+1], path[i])
+        ensures isAscTreePath(path, start, end)
+    {
+    }
+
+    lemma AscPathChildren(path: seq<Tree>, start: Tree, end: Tree)
+        requires start != Nil
+        requires end != Nil
+        requires |path| > 1
+        requires isAscTreePath(path, start, end)
+        ensures forall i :: 0 <= i < |path| - 1 ==> isChild(path[i+1], path[i])
+    {
+    }
+
+
+    lemma TreeSetChildInTreeSet(root: Tree, child: Tree) 
+        requires root != Nil
+        requires child != Nil && child in TreeSet(root)
+        ensures TreeSet(child) <= TreeSet(root)
+    {}
+
+    lemma parentNotInTreeSet(parent: Tree, root: Tree)
+        requires parent != Nil && parent != root && (parent.left == root || parent.right == root)
+        ensures parent !in TreeSet(root)
+    {
+        if root == Nil {} else {
+            assert TreeSet(root) == {root}+TreeSet(root.left)+TreeSet(root.right);
+            parentNotInTreeSet(root, root.left);
+            parentNotInTreeSet(root, root.right);
+            if parent in TreeSet(root.left) {
+                TreeSetChildInTreeSet(root.left, parent);
+            }else if parent in TreeSet(root.right) {
+                TreeSetChildInTreeSet(root.right, parent);
+            }
+        }
+    }
+
+
+    lemma childInTreeSet(root: Tree, child: Tree)
+        requires root != Nil && child != Nil
+        requires isChild(root, child)
+        ensures child in TreeSet(root)
+    {}
+
+    lemma validChildrenAlt(path: seq<Tree>, start: Tree, end: Tree)
+        requires start != Nil
+        requires end != Nil
+        requires |path| > 1
+        requires path[0] == start;
+        requires path[|path|-1] == end;
+        requires forall i :: 0 <= i < |path| ==> path[i] != Nil
+        requires forall i :: 0 <= i < |path| - 1 ==> isChild(path[i], path[i+1])
+        requires forall i :: 0 <= i < |path| - 1 ==> path[i+1] in TreeSet(path[i+1])
+        ensures forall i :: 0 <= i < |path| - 1 ==> isValidPath(path[i..], path[i])
+    {
+        if |path| == 2 {
+
+        }else{
+            validChildrenAlt(path[1..], path[1], end);
+        }
+    }
+
+    lemma isDescPathAndValidImpliesAllValid(path: seq<Tree>, start: Tree, end: Tree) 
+        requires isDescTreePath(path, start, end)
+        requires isValidPath(path, start)
+        requires |path| > 1
+        ensures forall i :: 0 <= i < |path| ==> isValidPath(path[i..], path[i]);
+    {
+        assert path[1] in TreeSet(start);
+        assert isDescTreePath(path[1..], path[1], end);
+        assert isValidPath(path[1..], start);
+        DescTreePathNotNil(path, start, end);
+        DescPathChildren(path, start, end);
+        assert forall i :: 0 <= i < |path| ==> path[i] in path;
+        validChildrenAlt(path, start, end);
+    }
+
+    lemma DescPathIsAscPath(path: seq<Tree>, start: Tree, end: Tree)
+        requires start != Nil
+        requires end != Nil
+        requires |path| >= 1
+        requires isDescTreePath(path, start, end)
+        ensures isAscTreePath(reverse(path), end, start)
+    {
+        DescTreePathNotNil(path, start, end);
+        ReverseIndexAll(path);
+        if |path| == 1 {} else {
+            DescPathChildrenReverse(path, start, end);
+            AscPathChildrenAlt(reverse(path), end, start);
+        }
+    }
+
+    lemma AscTreePathNotNil(path: seq<Tree>, start: Tree, end: Tree)
+        requires start != Nil
+        requires end != Nil
+        requires |path| >= 1
+        requires isAscTreePath(path, start, end)
+        ensures forall node :: node in path ==> node != Nil
+    {
+        if |path| == 1 {
+        }else if |path| > 1 {
+            assert path == [path[0]]+path[1..];
+            AscTreePathNotNil(path[1..], path[1], end);
+        }
+    }
+
+    lemma AscPathChildrenReverse(path: seq<Tree>, start: Tree, end: Tree)
+        requires start != Nil
+        requires end != Nil
+        requires |path| > 1
+        requires isAscTreePath(path, start, end)
+        ensures forall i :: 0 <= i < |reverse(path)| - 1 ==> isChild(reverse(path)[i], reverse(path)[i+1])
+    {
+        AscPathChildren(path, start, end);
+        ReverseIndexAll(path);
+    }
+
+    lemma AscPathIsDescPath(path: seq<Tree>, start: Tree, end: Tree)
+        requires start != Nil
+        requires end != Nil
+        requires |path| >= 1
+        requires isAscTreePath(path, start, end)
+        ensures isDescTreePath(reverse(path), end, start)
+    {
+        AscTreePathNotNil(path, start, end);
+        ReverseIndexAll(path);
+        // reversePreservesMultiset(path);
+        if |path| == 1 {
+
+        }else{
+            // assert path[0] == start;
+            // assert path[ |path| - 1] == end;
+            // assert reverse(path)[0] == end;
+            // assert reverse(path)[|path|-1] == start;
+            AscPathChildrenReverse(path, start, end);
+            // assert forall x :: x in reverse(path) ==> x in path && x != Nil;
+            assert forall i :: 0 <= i < |reverse(path)| ==> reverse(path)[i] in path && reverse(path)[i] != Nil;
+            DescPathChildrenAlt(reverse(path), end, start);
+        }
+    }
+
+    lemma DescPathPlusDescPath(path: seq<Tree>, start: Tree, middle: Tree, pathtwo: seq<Tree>, end: Tree)
+        requires start != Nil
+        requires end != Nil
+        requires middle != Nil
+        requires isDescTreePath(path, start, middle)
+        requires isDescTreePath(pathtwo, middle, end)
+        requires |path| > 1
+        requires |pathtwo| > 1
+        ensures isDescTreePath(path + pathtwo[1..], start, end)
+        ensures |path + pathtwo[1..]| == |path|+|pathtwo|-1;
+    {
+        DescPathChildren(path, start, middle);
+        DescPathChildren(pathtwo, middle, end);
+        DescTreePathNotNil(path, start, middle);
+        DescTreePathNotNil(pathtwo, middle, end);
+        assert forall i :: 0 <= i < |path| ==> path[i] in path;
+        assert forall i :: 0 <= i < |pathtwo| ==> pathtwo[i] in pathtwo;
+        DescPathChildrenAlt(path + pathtwo[1..], start, end);
+    }
+
+    lemma DescTreePathNoChildren(path: seq<Tree>, root: Tree, end: Tree)
+        requires root != Nil
+        requires end != Nil
+        requires |path| > 1
+        requires isDescTreePath(path, root, end)
+        ensures forall x :: x in path[1..] ==> x in TreeSet(root) - {root} 
+    {
+        if |path| == 2 {
+        }else{
+            if root.left != Nil && isDescTreePath(path[1..], root.left, end) {
+                parentNotInTreeSet(root,root.left);
+                forall x | x in path[1..] 
+                    ensures x in TreeSet(root) - {root}
+                {
+                    assert path[1..] == [path[1]]+path[2..];
+                }
+            }else if root.right != Nil && isDescTreePath(path[1..], root.right, end) {
+                parentNotInTreeSet(root,root.right);
+                forall x | x in path[1..] 
+                    ensures x in TreeSet(root) - {root}
+                {
+                    assert path[1..] == [path[1]] + path[2..];
+                } 
+            }
+        }
+    }
+
+    lemma DescTreePathInjective(path: seq<Tree>, root: Tree, end: Tree)
+        requires root != Nil
+        requires end != Nil
+        requires isDescTreePath(path, root, end)
+        ensures distinct(path)
+    {
+        if |path| == 1 {
+
+        }else{
+            assert path[1] == root.left || path[1] == root.right;
+            assert root != root.left && root != root.right;
+            assert path == [root]+path[1..];
+            var rest := path[1..];
+            DescTreePathInjective(rest,path[1], end);
+            assert distinct(rest);
+            DescTreePathNoChildren(path, root, end);
+            forall x,y | x != y && 0 <= x <= y < |path| 
+                ensures path[x] != path[y]; 
+            {
+                if x == 0 {
+                    assert path[x] == root;
+                    assert path[y] in path[1..];
+                    assert path[y] != root;
+                }else{
+                    assert path[x] != path[y];
+                }
+            }
+        }
+    }
+
+    lemma DescTreePathToPath(path: seq<Tree>, root: Tree, end: Tree)
+        requires root != Nil
+        requires end != Nil
+        requires isDescTreePath(path, root, end)
+        ensures isTreePath(path, root, end)
+    {
+        assert path[0] == root;
+        assert path[|path|-1] == end;
+        if |path| == 1 {
+            assert path == [root];
+            assert isDescTreePath([root], root, end);
+            assert root == end;
+            assert isTreePath([root], root, end);
+        }
+    }
+
+    lemma AscTreePathToPath(path: seq<Tree>, root: Tree, end: Tree)
+        requires root != Nil
+        requires end != Nil
+        requires isAscTreePath(path, root, end)
+        ensures isTreePath(path, root, end)
+    {
+        assert path[0] == root;
+        assert path[|path|-1] == end;
+        if |path| == 1 {
+            assert path == [root];
+            assert isAscTreePath([root], root, end);
+            assert root == end;
+            assert isTreePath([root], root, end);
+        }
+    }
+
+    lemma DescTreePathNotNil(path: seq<Tree>, start: Tree, end: Tree)
+        requires start != Nil
+        requires end != Nil
+        requires |path| >= 1
+        requires isDescTreePath(path, start, end)
+        ensures forall node :: node in path ==> node != Nil
+        ensures forall i :: 0 <= i < |path| ==> path[i] != Nil
+    {
+        if |path| == 1 {
+        }else if |path| > 1 {
+            assert path == [path[0]]+path[1..];
+            DescTreePathNotNil(path[1..], path[1], end);
+        }
+    }
+
+    lemma TreePathNotNil(path: seq<Tree>, start: Tree, end: Tree)
+        requires start != Nil
+        requires |path| >= 1
+        requires isTreePath(path, start, end)
+        ensures forall node :: node in path ==> node != Nil
+        ensures forall i :: 0 <= i < |path| ==> path[i] != Nil
+    {
+        if |path| == 1 {
+        }else if |path| > 1 {
+            assert path == [path[0]]+path[1..];
+            TreePathNotNil(path[1..], path[1], end);
+        }
+    }
+
+    lemma TreePlusTree(path: seq<Tree>, start: Tree, root: Tree, pathtwo: seq<Tree>, end: Tree)
+        requires start != Nil && root != Nil && end != Nil
+        requires start != root && root != end
+        requires isTreePath(path, start, root)
+        requires isTreePath(pathtwo, root, end)
+        ensures isTreePath(path + pathtwo[1..], start, end)
+        ensures |path + pathtwo[1..]| == |path|+|pathtwo|-1
+    {
+        TreePathsAreTheSameAlt(path, start, root);
+        TreePathsAreTheSameAlt(pathtwo, root, end);
+        assert isTreePathAlt(path + pathtwo[1..], start, end);
+        TreePathsAreTheSame(path + pathtwo[1..], start, end);
+    }
+
+    lemma DescPlusAsc(path: seq<Tree>, start: Tree, root: Tree, pathtwo: seq<Tree>, end: Tree)
+        requires start != Nil && root != Nil && end != Nil
+        requires start != root && root != end
+        requires isDescTreePath(path, root, end)
+        requires isAscTreePath(pathtwo, start, root)
+        ensures isTreePath(pathtwo + path[1..], start, end)
+    {
+        var result := pathtwo + path[1..];
+        assert result[0] == start;
+        DescTreePathToPath(path, root, end);
+        AscTreePathToPath(pathtwo, start, root);
+        TreePlusTree(pathtwo, start, root, path, end);
+        assert |pathtwo + path[1..]| == |pathtwo| + |path| -1;
+    }
+
+    lemma DescPlusDesc(path: seq<Tree>, start: Tree, root: Tree, pathtwo: seq<Tree>, end: Tree)
+        requires start != Nil && root != Nil && end != Nil
+        requires start != root && root != end
+        requires isDescTreePath(path, root, end)
+        requires isDescTreePath(pathtwo, root, start)
+        ensures isTreePath(reverse(pathtwo) + path[1..], start, end)
+    {
+        DescPathIsAscPath(pathtwo, root, start);
+        assert isAscTreePath(reverse(pathtwo), start, root);
+        DescPlusAsc(path, start, root, reverse(pathtwo), end);
+    }
+
+
+    lemma isPathSlices(path: seq<Tree>, start: Tree, end: Tree, root: Tree) 
+        requires |path| >= 1
+        requires isPath(path, start, end, root)
+        ensures forall i :: 0 < i < |path| ==> isPath(path[..(i+1)], start, path[i], root) && isPath(path[i..], path[i], end, root)
+    {
+        TreePathNotNil(path, start, end);
+        TreePathsAreTheSameAlt(path, start, end);
+        forall i | 0 < i < |path| 
+            ensures isPath(path[..(i+1)], start, path[i], root) && isPath(path[i..], path[i], end, root)
+        {
+            assert path == path[..i]+path[i..];
+            TreePathChildrenAlt(path[..(i+1)], start, path[i]);
+            TreePathChildrenAlt(path[i..], path[i], end);
+            assert isValidPath(path[..i], root);
+            assert isValidPath(path[i..], root);
+            assert distinct(path[..i]);
+            assert distinct(path[i..]);
+        }
+    }
+
+    lemma notRootNotDesc(root: Tree, start: Tree, end: Tree, path: seq<Tree>)
+        requires isValidPath(path, root)
+        requires root in path
+        ensures start != root ==> !isDescTreePath(path, start, end)
+    {
+        if isDescTreePath(path, start, end) {
+            descRoot(root, start, end, path);
+        }
+    }
+
+    lemma descRoot(root: Tree, start: Tree, end: Tree, path: seq<Tree>) 
+        requires isDescTreePath(path, start, end)
+        requires isValidPath(path, root)
+        requires root in path
+        ensures start == root
+    {
+        if start == root {
+
+        }else {
+            assert path[0] != root;
+            assert path == [path[0]]+path[1..];
+            assert root in path[1..];
+            DescPathChildren(path, start, end);
+            var i :| 0 < i< |path| && path[i] == root;
+            assert isChild(path[i-1], root);
+            parentNotInTreeSet(path[i-1], root);
+            assert false;
+        }
+    }
+
+    lemma LastNotRootNotAsc(root: Tree, start: Tree, end: Tree, path: seq<Tree>)
+        requires isValidPath(path, root)
+        requires root in path
+        ensures end != root ==> !isAscTreePath(path, start, end)
+    {
+        if isAscTreePath(path, start, end) {
+            ascRoot(root, start, end, path);
+        }
+    }
+
+    lemma ascRoot(root: Tree, start: Tree, end: Tree, path: seq<Tree>)
+        requires isAscTreePath(path, start, end)
+        requires isValidPath(path, root)
+        requires root in path
+        ensures end == root
+    {
+        if end == root {
+
+        }else {
+            assert path[|path|-1] != root;
+            AscPathChildren(path,start,end);
+            var i :| 0 <= i < |path|-1 && path[i] == root;
+            assert isChild(path[i+1], path[i]);
+            parentNotInTreeSet(path[i+1], root);
+            assert false;
+        }
+    }
+
+    lemma TreeHeightToDescTreePath(root: Tree, h: int) 
+        requires root != Nil
+        requires h == TreeHeight(root)
+        ensures exists end: Tree, path: seq<Tree> :: (isLeaf(end) && end in TreeSet(root))  && isDescTreePath(path, root, end) && |path| == h+1 && isValidPath(path, root) && distinct(path)
+    {
+        if h == 0 {
+            assert isDescTreePath([root], root, root);
+            assert isValidPath([root], root);
+            assert distinct([root]);
+            assert root in TreeSet(root);
+        }else if h >= 1 {
+            if root.left != Nil && TreeHeight(root.left) == h-1 {
+                TreeHeightToDescTreePath(root.left, h-1);
+                TreeSetChildInTreeSet(root, root.left);
+                var end: Tree, path: seq<Tree> :| isLeaf(end) && end in TreeSet(root.left) && isDescTreePath(path, root.left, end) && |path| == h && isValidPath(path, root.left) && distinct(path);
+                assert end != Nil && isDescTreePath([root]+path, root, end) && |[root]+path| == h+1;
+                parentNotInTreeSet(root, root.left);
+                distincts([root], path);
+                assert distinct([root]+path);
+                assert isValidPath([root]+path, root);
+            } else if root.right != Nil && TreeHeight(root.right) == h-1 {
+                TreeHeightToDescTreePath(root.right, h-1);
+                TreeSetChildInTreeSet(root, root.right);
+                var end: Tree, path: seq<Tree> :| isLeaf(end) && end in TreeSet(root.right) && isDescTreePath(path, root.right, end) && |path| == h && isValidPath(path, root.right) && distinct(path);
+                assert end != Nil && isDescTreePath([root]+path, root, end) && |[root]+path| == h+1;
+                parentNotInTreeSet(root, root.right);
+                distincts([root], path);
+                assert distinct([root]+path);
+                assert isValidPath([root]+path, root);
+            }
+        }
+    }
+
+    lemma parentsAreTheSame(p1: Tree, p2: Tree, child: Tree)
+        requires p1 != Nil && p2 != Nil && child != Nil
+        requires isChild(p1, child)
+        requires isChild(p2, child)
+        ensures p1 == p2
+
+    lemma pathStartingAtRootDescSlice(root: Tree, start: Tree, end: Tree, path: seq<Tree>, i: int)
+        requires root != Nil
+        requires root in path && path[0] == root
+        requires ChildrenAreSeparate(root)
+        requires isPath(path, start, end, root)
+        requires 0 < i <= |path|
+        requires isDescTreePath(path[0..i], root, path[i-1])
+        requires |path| >= 1
+        decreases |path| - i
+        ensures isDescTreePath(path, root, end)
+    {
+        TreePathNotNil(path, start, end);
+        TreePathsAreTheSameAlt(path, start,end);
+        if i < |path| {
+            if isChild(path[i-1], path[i]) {
+                if i == 1 {
+                    assert isDescTreePath(path[0..1], root, path[i-1]);
+                }else{
+
+                    DescPathChildren(path[0..i], root, path[i-1]);
+                }
+                DescPathChildrenAlt(path[0..(i+1)], root, path[i]);
+                assert isDescTreePath(path[0..(i+1)], root, path[i]);
+                pathStartingAtRootDescSlice(root, start, end, path, i+1);
+            }else if isChild(path[i], path[i-1]) {
+                if i == 1 {
+                    parentNotInTreeSet(path[i],root);
+                }else{
+                    DescPathChildren(path[0..i], root, path[i-1]);
+                    assert isChild(path[i-2],path[i-1]);
+                    parentsAreTheSame(path[i-2], path[i], path[i-1]);
+                    assert path[i-2] == path[i];
+                    assert false;
+                }
+                assert false;
+            }else{
+                assert !isParentOrChild(path[i-1], path[i]);
+                assert false;
+            }
+        }else{
+            assert i == |path|;
+            assert isDescTreePath(path[0..|path|], root, path[|path|-1]);
+            assert path[0..|path|] == path;
+        }
+    }
+
+    lemma pathStartingAtRootDesc(root: Tree, start: Tree, end: Tree, path: seq<Tree>)
+        requires root != Nil
+        requires root in path && path[0] == root
+        requires ChildrenAreSeparate(root)
+        requires isPath(path, start, end, root)
+        requires |path| >= 1
+        decreases |path|
+        ensures isDescTreePath(path, root, end)
+    {
+        if |path| == 1 {
+
+        }else{
+            if isChild(path[1], root) {
+                parentNotInTreeSet(path[1], root);
+                assert false;
+            }else if isChild(root, path[1]) {
+                assert path[1] == root.left || path[1] == root.right;
+                assert isDescTreePath([root, path[1]], root, path[1]);
+                pathStartingAtRootDescSlice(root, start, end, path, 1);
+            }
+        }
+    }
+
 }
